iris/ProofPipealloc.v
@@ -28,7 +28,7 @@ From Stdlib Require Import Eqdep_dec ZArith Lia List.
 From stdpp Require Import gmap list list_monad bitvector.definitions bitvector.tactics.
 From iris.proofmode Require Import proofmode.
 From iris.algebra Require Import excl auth gmap frac numbers.
-From iris.base_logic.lib Require Import cancelable_invariants ghost_var gen_heap invariants.
+From iris.base_logic.lib Require Import ghost_var gen_heap invariants.
 From iris.program_logic Require Import language weakestpre lifting.
 Require Import SailStdpp.ConcurrencyInterface SailStdpp.ConcurrencyInterfaceBuiltins SailStdpp.ConcurrencyInterfaceTypes SailStdpp.Operators_mwords.
 Require Import Riscv.rv64d_types Riscv.rv64d Riscv.riscv_extras.
@@ -86,7 +86,7 @@ Module PipeallocProof (Filealloc : FILEALLOC) (Kalloc : KALLOC)
                       (Initlock : INITLOCK) (Fileclose : FILECLOSE) : PIPEALLOC.
 
 Section ProofPipealloc.
-  Context `{!riscvGS Σ, !lockG Σ, !sieG Σ, !fileG Σ, !fdslotG Σ, !kallocG Σ, !pipeG Σ, !cinvG Σ}.
+  Context `{!riscvGS Σ, !lockG Σ, !sieG Σ, !fileG Σ, !fdslotG Σ, !kallocG Σ, !pipeG Σ}.
   Context `{CID : CpuId}.
 
   Notation PA := KernelSyms.pipealloc.
